concrete/exec.v
@@ -24,8 +24,8 @@ Local Notation "x .+1" := (x + Z_to_word 1).
 
 Definition step (st : state mt) : option (state mt) :=
   let 'mkState mem reg cache pc@tpc epc := st in
-  do i <- PartMaps.get mem pc;
-  do instr <- decode_instr (val i);
+  do! i <- PartMaps.get mem pc;
+  do! instr <- decode_instr (val i);
   let mvec := mkMVec (op_to_word (opcode_of instr)) tpc (tag i) in
   match instr with
   | Nop =>
@@ -48,17 +48,17 @@ Definition step (st : state mt) : option (state mt) :=
     next_state_reg _ masks st mvec r3 (binop_denote f (val v1) (val v2))
   | Load r1 r2 =>
     let v1 := TotalMaps.get reg r1 in
-    do v2 <- PartMaps.get mem (val v1);
+    do! v2 <- PartMaps.get mem (val v1);
     let old := TotalMaps.get reg r2 in
     let mvec := mvec (tag v1) (tag v2) (tag old) in
     next_state_reg _ masks st mvec r2 (val v2)
   | Store r1 r2 =>
     let v1 := TotalMaps.get reg r1 in
     let v2 := TotalMaps.get reg r2 in
-    do v3 <- PartMaps.get mem (val v1);
+    do! v3 <- PartMaps.get mem (val v1);
     let mvec := mvec (tag v1) (tag v2) (tag v3) in
     next_state _ masks st mvec (fun rvec =>
-      do mem' <- PartMaps.upd mem (val v1) (val v2)@(ctr rvec);
+      do! mem' <- PartMaps.upd mem (val v1) (val v2)@(ctr rvec);
       Some (mkState mem' reg cache (pc.+1)@(ctrpc rvec) epc))
   | Jump r =>
     let v := TotalMaps.get reg r in
@@ -80,7 +80,7 @@ Definition step (st : state mt) : option (state mt) :=
   | AddRule =>
     let mvec := mvec TNone TNone TNone in
     next_state _ masks st mvec (fun rvec =>
-      do cache' <- add_rule ops cache masks (is_kernel_tag tpc) mem;
+      do! cache' <- add_rule ops cache masks (is_kernel_tag tpc) mem;
       Some (mkState mem reg cache' epc epc))
   | GetTag r1 r2 =>
     let v1 := TotalMaps.get reg r1 in
@@ -118,7 +118,7 @@ Proof.
 
     (* Invert all binds *)
     repeat match goal with
-             | STEP : (do x <- ?t; _) = Some _ |- _ =>
+             | STEP : (do! x <- ?t; _) = Some _ |- _ =>
                destruct t eqn:?; simpl in STEP; try discriminate
              | x : atom _ _ |- _ =>
                destruct x; simpl in *
@@ -145,7 +145,7 @@ Fixpoint stepn (max_steps : nat) (st : state mt) : option (state mt) :=
   match max_steps with
   | O => Some st
   | S max_steps' =>
-    do st' <- step st;
+    do! st' <- step st;
     stepn max_steps' st'
   end.
 
